thy/LevelCollapse.thy
@@ -1,0 +1,93 @@
+theory LevelCollapse
+imports Conc_Impl
+begin
+
+definition "bddmi_rel cs \<equiv> {(a,c)|a b c. (a,b) \<in> bf_ifex_rel \<and> (c,b) \<in> Rmi cs \<and> bdd_sane cs}"
+definition "bdd_relator a d s \<equiv> \<exists>\<^sub>Acs. is_bdd_impl cs s * \<up>(in_rel (bddmi_rel cs) a d)"
+(* I know, I know\<dots> *)
+
+thm bdd_relator_def[unfolded bddmi_rel_def, simplified]
+lemma join_hlp1: "is_bdd_impl a s * is_bdd_impl b s \<Longrightarrow>\<^sub>A is_bdd_impl a s * is_bdd_impl b s * \<up>(a = b)"
+unfolding is_bdd_impl_def
+apply clarsimp
+apply(rule preciseD[where p=s and R="is_pointermap_impl" and F="is_pointermap_impl b s" and F'="is_pointermap_impl a s"])
+apply(rule is_pointermap_impl_prec)
+apply(unfold mod_and_dist)
+apply(rule conjI)
+apply assumption
+apply(simp add: star_aci(2))
+done
+
+lemma join_hlp: "is_bdd_impl a s * is_bdd_impl b s = is_bdd_impl b s * is_bdd_impl a s * \<up>(a = b)"
+	apply(rule ent_iffI[rotated])
+	apply simp
+	apply(rule ent_trans)
+	 apply(rule join_hlp1)
+	apply(simp)
+done
+
+lemma add_true_asm:
+	assumes "<b * true> p <a>\<^sub>t"
+	shows "<b> p <a>\<^sub>t"
+	apply(rule cons_pre_rule)
+	prefer 2
+	apply(rule assms)
+	apply(simp add: ent_true_drop)
+done
+
+lemma add_anything:
+	assumes "<b> p <a>"
+	shows "<b * x> p <\<lambda>r. a r * x>\<^sub>t"
+proof -
+	note [sep_heap_rules] = assms
+	show ?thesis by sep_auto
+qed
+
+lemma add_true:
+	assumes "<b> p <a>\<^sub>t"
+	shows "<b * true> p <a>\<^sub>t"
+	using assms add_anything[where x=true] by force
+
+thm iteci_rule[THEN mp] brofix.ite_impl_R ifex_ite_rel_bf
+(* Yeah, this is rubbish. *)
+lemma "
+<bdd_relator ib ic s * bdd_relator tb tc s * bdd_relator eb ec s> 
+	iteci ic tc ec s
+<\<lambda>(r,s'). bdd_relator (bf_ite ib tb eb) r s'>\<^sub>t"
+	apply(unfold bdd_relator_def)
+	apply(simp)
+	apply(intro norm_pre_ex_rule)
+	apply(clarsimp)
+	apply(unfold bddmi_rel_def)
+	apply(rename_tac cse cst csi)
+	apply(unfold star_assoc)
+	apply(subst join_hlp)
+	apply(unfold star_assoc[symmetric])
+	apply(subst join_hlp)
+	apply(clarsimp)
+	apply(drule (3) brofix.ite_impl_R[where ii=ic and ti=tc and ei=ec, unfolded in_rel_def])
+	apply(drule ospecD2)
+	apply(clarsimp simp del: ifex_ite.simps)
+	apply(rule cons_post_rule)
+	 apply(rule cons_pre_rule)
+	  prefer 2
+	  apply(rule iteci_rule[THEN mp, THEN add_true])
+	  apply(assumption)
+	 apply(sep_auto)
+	apply(clarsimp simp del: ifex_ite.simps)
+	apply(rule ent_ex_postI)
+	apply(subst ent_pure_post_iff)
+	apply(rule conjI)
+	 prefer 2
+	 apply(sep_auto)
+	apply(clarsimp simp del: ifex_ite.simps)
+	apply(rule exI)
+	apply(rule conjI)
+	 apply(erule (2) ifex_ite_rel_bf[unfolded in_rel_def])
+	apply assumption
+done
+
+(* Todo: Verify all of these\<dots> *)
+export_code open iteci notci andci orci ifci tci fci emptyci in Haskell file "output"
+
+end
